unfold sq

code/ecdsap256sha2/Hacl.Impl.LowLevel.fst
@@ -684,31 +684,141 @@ let sq0 f result =
   let o1 = sub result (size 1) (size 1) in 
   let o2 = sub result (size 2) (size 1) in 
   let o3 = sub result (size 3) (size 1) in 
-    
-    let h0 = ST.get() in 
+
   mul64 f0 f0 o0 temp;
-
-
-    let h1 = ST.get() in 
-  
-  (*let c1 = mult64_c f1 f0 (u64 0) o1 temp in  *)
   
   let h = index temp (size 0) in 
-  mul64 f1 f0 o1 temp;
+  mul64 f0 f1 o1 temp;
   let l = index o1 (size 0) in     
   let c1 = add_carry_u64 (u64 0) l h o1 in 
 
+  let h = index temp (size 0) in 
+  mul64 f0 f2 o2 temp;
+  let l = index o2 (size 0) in     
+  let c2 = add_carry_u64 c1 l h o2 in
+  
+  let h = index temp (size 0) in 
+  mul64 f0 f3 o3 temp;
+  let l = index o3 (size 0) in     
+  let c3 = add_carry_u64 c2 l h o3 in
 
-
-    let h2 = ST.get() in 
-  let c2 = mult64_c f2 f0 c1 o2 temp in 
-    let h3 = ST.get() in 
-  let c3 = mult64_c f3 f0 c2 o3 temp in 
-    let h4 = ST.get() in 
   let temp0 = index temp (size 0) in 
 
   pop_frame();  
   c3 +! temp0
+
+
+
+
+val sq1: f1: felem -> f3: felem -> result: felem -> 
+  Stack uint64 
+  (requires fun h -> live h f1 /\ live h f3 /\ live h result /\ eq_or_disjoint f3 result /\ disjoint f1 result)
+  (ensures fun h0 c h1 -> modifies (loc result) h0 h1)
+
+let sq1 f_ f4 result = 
+  push_frame();
+    let result_ = create (size 4) (u64 0) in 
+  let temp = create (size 1) (u64 0) in 
+
+  let f0 = index f_ (size 0) in 
+  let f1 = index f_ (size 1) in 
+  let f2 = index f_ (size 2) in 
+  let f3 = index f_ (size 3) in 
+    
+  let o0 = sub result_ (size 0) (size 1) in 
+  let o1 = sub result_ (size 1) (size 1) in 
+  let o2 = sub result_ (size 2) (size 1) in 
+  let o3 = sub result_ (size 3) (size 1) in 
+
+
+  mul64 f0 f1 o0 temp;
+
+ 
+  let h = index temp (size 0) in 
+  mul64 f1 f1 o1 temp;
+  let l = index o1 (size 0) in     
+  let c1 = add_carry_u64 (u64 0) l h o1 in 
+
+  let h = index temp (size 0) in 
+  mul64 f1 f2 o2 temp;
+  let l = index o2 (size 0) in     
+  let c2 = add_carry_u64 c1 l h o2 in
+  
+  let h = index temp (size 0) in 
+  mul64 f1 f3 o3 temp;
+  let l = index o3 (size 0) in     
+  let c3 = add_carry_u64 c2 l h o3 in
+
+  let temp0 = index temp (size 0) in 
+  
+  let c = c3 +! temp0 in 
+
+
+  let c3 = add4 result_ f4 result in 
+  admit();
+  pop_frame();  
+  c +! c3
+
+
+
+
+
+val sq2: f1: felem -> f3: felem -> result: felem -> 
+  Stack uint64 
+  (requires fun h -> live h f1 /\ live h f3 /\ live h result /\ eq_or_disjoint f3 result /\ disjoint f1 result)
+  (ensures fun h0 c h1 -> modifies (loc result) h0 h1)
+
+let sq2 f_ f4 result = 
+  push_frame();
+    let result_ = create (size 4) (u64 0) in 
+  let temp = create (size 1) (u64 0) in 
+
+  let f0 = index f_ (size 0) in 
+  let f1 = index f_ (size 1) in 
+  let f2 = index f_ (size 2) in 
+  let f3 = index f_ (size 3) in 
+    
+  let o0 = sub result_ (size 0) (size 1) in 
+  let o1 = sub result_ (size 1) (size 1) in 
+  let o2 = sub result_ (size 2) (size 1) in 
+  let o3 = sub result_ (size 3) (size 1) in 
+
+
+  mul64 f0 f2 o0 temp;
+
+ 
+  let h = index temp (size 0) in 
+  mul64 f1 f2 o1 temp;
+  let l = index o1 (size 0) in     
+  let c1 = add_carry_u64 (u64 0) l h o1 in 
+
+  let h = index temp (size 0) in 
+  mul64 f2 f2 o2 temp;
+  let l = index o2 (size 0) in     
+  let c2 = add_carry_u64 c1 l h o2 in
+  
+  let h = index temp (size 0) in 
+  mul64 f2 f3 o3 temp;
+  let l = index o3 (size 0) in     
+  let c3 = add_carry_u64 c2 l h o3 in
+
+  let temp0 = index temp (size 0) in 
+  
+  let c = c3 +! temp0 in 
+
+
+  let c3 = add4 result_ f4 result in 
+  admit();
+  pop_frame();  
+  c +! c3
+
+
+
+
+
+
+
+
 
 
 
@@ -732,17 +842,20 @@ let sq f r out =
   let c0 = sq0 r b0 in 
     upd temp (size 4) c0;
 
+
+
+
     let h1 = ST.get() in 
     let bk0 = sub temp (size 0) (size 1) in 
   let b1 = sub temp (size 1) (size 4) in   
-  let c1 = mul1_add r f1 b1 b1 in 
+  let c1 = sq1 r b1 b1 in 
       upd temp (size 5) c1; 
     let h2 = ST.get() in
       assert(Lib.Sequence.index (as_seq h1 bk0) 0 == Lib.Sequence.index (as_seq h1 temp) 0);
 
       let bk1 = sub temp (size 0) (size 2) in 
   let b2 = sub temp (size 2) (size 4) in 
-  let c2 = mul1_add r f2 b2 b2 in 
+  let c2 = sq2 r b2 b2 in 
     upd temp (size 6) c2;
     
     let h3 = ST.get() in 
